progs/verif_tree.v
@@ -549,16 +549,13 @@ Context {V: Type}.
 Variable listrep: list V -> val -> mpred.
 
 Definition lseg (contents: list V) (x z: val) : mpred :=
-  ALL tcontents: list V, listrep tcontents z -* listrep (contents ++ tcontents) x.
+  ALL tcontents: list V, (listrep tcontents z -* listrep (contents ++ tcontents) x).
 
 Lemma emp_lseg_nil: forall (x: val),
   emp |-- lseg nil x x.
 Proof.
-  intros.
-  apply allp_right; intros.
-  apply wand_sepcon_adjoint.
-  simpl.
-  entailer!.
+  unfold lseg.
+  auto.
 Qed.
 
 Lemma lseg_lseg: forall (s1 s2: list V) (x y z: val),
@@ -566,12 +563,8 @@ Lemma lseg_lseg: forall (s1 s2: list V) (x y z: val),
 Proof.
   intros.
   unfold lseg.
-  eapply derives_trans; [apply sepcon_derives; [apply derives_refl |] | apply wandQ_frame_ver].
-  eapply derives_trans; [apply (wandQ_frame_refine _ _ _ (app s2)) |].
-  apply derives_refl'.
-  f_equal; extensionality tcontents; simpl.
-  rewrite app_assoc.
-  auto.
+  iIntros "(H2 & H1)" (?) "H".
+  rewrite <- app_assoc; iApply "H1"; iApply "H2"; done.
 Qed.
 
 Lemma list_lseg: forall (s1 s2: list V) (x y: val),
@@ -579,13 +572,7 @@ Lemma list_lseg: forall (s1 s2: list V) (x y: val),
 Proof.
   intros.
   unfold lseg.
-  change (listrep s2 y) with ((fun s2 => listrep s2 y) s2).
-   change
-     (ALL tcontents : list V, listrep tcontents y -* listrep (s1 ++ tcontents) x)
-   with
-     (allp ((fun tcontents => listrep tcontents y) -* (fun tcontents => listrep (s1 ++ tcontents) x))).
-   change (listrep (s1 ++ s2) x) with ((fun s2 => listrep (s1 ++ s2) x) s2).
-   apply wandQ_frame_elim.
+  iIntros "(? & H)"; iApply "H"; done.
 Qed.
 
 End GeneralLseg.
@@ -598,8 +585,6 @@ Proof.
   {
     forward.
     entailer!.
-    simpl.
-    auto.
   }
   unfold Sfor.
   destruct t as [| tl v].
@@ -625,19 +610,19 @@ Proof.
       LOCAL (temp _q q)
       SEP (data_at Tsh t_struct_Xnode (q_root, Vint (Int.repr (v + 1))) p;
            GeneralLseg.lseg (list_rep (fun p n q : val => data_at Tsh t_struct_Xlist (p, n) q)) (map snd tl1) q_root q;
-           iter_sepcon (uncurry xtree_rep) tl1;
+           [∗ list] x ∈ tl1, uncurry xtree_rep x;
            list_rep (fun p n q : val => data_at Tsh t_struct_Xlist (p, n) q) (map snd tl2) q;
-           iter_sepcon (uncurry xtree_rep) tl2))%assert
+           [∗ list] x ∈ tl2, uncurry xtree_rep x))%assert
   break:
     ( PROP ()
       LOCAL ()
       SEP (data_at Tsh t_struct_Xnode (q_root, Vint (Int.repr (v + 1))) p;
            list_rep (fun p n q : val => data_at Tsh t_struct_Xlist (p, n) q) (map snd tl) q_root;
-           iter_sepcon (uncurry xtree_rep) (map (fun tp => (x_add1 (fst tp), snd tp)) tl)))%assert.
+           [∗ list] x ∈ (map (fun tp => (x_add1 (fst tp), snd tp)) tl), uncurry xtree_rep x))%assert.
   {
     Exists (@nil (XTree * val)) tl q_root.
     entailer!!.
-    apply GeneralLseg.emp_lseg_nil.
+    rewrite <- GeneralLseg.emp_lseg_nil; auto.
   }
   {
     Intros tl1 tl2 q.
@@ -650,7 +635,6 @@ Proof.
       simpl in H0; rewrite app_nil_r in H0.
       simpl map.
       sep_apply (GeneralLseg.list_lseg (list_rep (fun p0 n q : val => data_at Tsh t_struct_Xlist (p0, n) q)) (map snd tl1) nil q_root nullval).
-      sep_apply (eq_sym (iter_sepcon_app (uncurry xtree_rep) tl1 [])).
       rewrite !app_nil_r.
       rewrite <- H0, map_map.
       simpl. change (fun x : XTree * val => snd x) with (@snd XTree val).
@@ -662,7 +646,7 @@ Proof.
       Intros.
       contradiction.
     }
-    simpl list_rep; simpl iter_sepcon.
+    simpl list_rep; simpl big_opL.
     Intros q'.
     change (uncurry xtree_rep (t, p')) with (xtree_rep t p').
     forward.
@@ -672,16 +656,14 @@ Proof.
     entailer!!.
     + rewrite <- app_assoc; auto.
     + change (xtree_rep (x_add1 t) p') with (uncurry xtree_rep (x_add1 t, p')).
-      rewrite iter_sepcon_app; simpl.
+      rewrite big_sepL_app; simpl.
       cancel.
       eapply derives_trans; [| rewrite map_app; apply (GeneralLseg.lseg_lseg _ _ _ _ q)].
       cancel.
       clear.
       apply allp_right; intros.
-      apply wand_sepcon_adjoint.
-      simpl list_rep.
-      Exists q'.
-      cancel.
+      iIntros "??"; simpl.
+      iExists q'; iFrame.
   }
   entailer!!.
   Exists q_root. cancel.
@@ -689,7 +671,7 @@ Proof.
   cancel.
   rewrite iter_sepcon2_spec.
   Exists (map (fun tp : XTree * val => (x_add1 (fst tp), snd tp)) tl); cancel.
-  entailer!!.
+  entailer!!; auto.
   rewrite !map_map.
   split; f_equal.
 Qed.
