floyd/proofauto.v
@@ -126,6 +126,8 @@ Global Arguments Qp.mul : simpl nomatch.
 Global Arguments Qp.inv : simpl nomatch.
 Global Arguments Qp.div : simpl nomatch.
 
+Global Instance inhabitant_inhabited `{Inhabitant A} : Inhabited A := populate default.
+
 (*funspec scope is the default, so remains open.
   Users who want to use old funspecs should 
   "Require Import Require Import VST.floyd.Funspec_old_Notation."
