progs/verif_queue2.v
@@ -153,7 +153,7 @@ Proof.
     + forward. subst p. congruence.
     + Intros. forward. entailer!.
 *
-  forward. Exists p; entailer!.
+  forward.
 Qed.
 
 Lemma fifo_isptr: forall al q, fifo al q |-- !! isptr q.
@@ -199,7 +199,7 @@ Qed.
 Lemma body_fifo_new: semax_body Vprog Gprog f_fifo_new fifo_new_spec.
 Proof.
   start_function.
-
+  rename a into gv.
   forward_call (* Q = surely_malloc(sizeof ( *Q)); *)
      (t_struct_fifo, gv).
   Intros q.
@@ -306,6 +306,7 @@ Qed.
 Lemma body_make_elem: semax_body Vprog Gprog f_make_elem make_elem_spec.
 Proof.
 start_function.
+rename a into gv.
 forward_call (*  p = surely_malloc(sizeof ( *p));  *)
     (t_struct_elem, gv).
 Intros p.
@@ -319,6 +320,7 @@ Qed.
 Lemma body_main:  semax_body Vprog Gprog f_main main_spec.
 Proof.
 start_function.
+rename a into gv.
 sep_apply (create_mem_mgr gv).
 forward_call (* Q = fifo_new(); *)  gv.
 Intros q.
