progs/verif_strlib.v
@@ -139,13 +139,13 @@ Qed.
 Lemma split_data_at_app_tschar:
  forall sh n (al bl: list val) p ,
    n = Zlength (al++bl) ->
-   data_at sh (tarray tschar n) (al++bl) p = 
+   data_at sh (tarray tschar n) (al++bl) p ⊣⊢
          data_at sh (tarray tschar (Zlength al)) al p
         * data_at sh (tarray tschar (n - Zlength al)) bl
                  (field_address0 (tarray tschar n) [ArraySubsc (Zlength al)] p).
 Proof.
 intros.
-apply (split2_data_at_Tarray_app _ n  sh tschar al bl ); auto.
+apply (split2_data_at_Tarray_app _ n  sh tschar al bl); auto.
 rewrite Zlength_app in H.
 change ( Zlength bl = n - Zlength al); lia.
 Qed.
@@ -224,8 +224,7 @@ forward_loop (EX i : Z,
       cancel.
     assert (j = Zlength ls) by cstring; subst.
     autorewrite with sublist.
-    apply derives_refl'.
-    unfold data_at; f_equal. 
+    f_equiv.
     replace (n - (Zlength ld + Zlength ls))
      with (1 + (n - (Zlength ld + Zlength ls+1))) by rep_lia.
     rewrite <- repeat_app' by rep_lia.
