sha/verif_sha_bdo8.v
@@ -4,7 +4,6 @@ Require Import sha.SHA256.
 Require Import sha.spec_sha.
 Require Import sha.sha_lemmas.
 Require Import sha.bdo_lemmas.
-Local Open Scope logic.
 
 Definition load8 id ofs :=
  (Sset id
